|   PDF/PMF    | Discrete                                                     | Continuous                                                   |
| :----------: | ------------------------------------------------------------ | ------------------------------------------------------------ |
|  **Joint**   | $p_{X,Y}(x, y) = P(X = x, Y = y)$<br />$\displaystyle P((X,Y)\in A) = \mathop{\sum\sum}_{(x, y) \in A}P(X = x, Y = y)$ | $\displaystyle f_{X, Y}(x, y) = \frac{\partial^2}{\partial x \partial y}F_{X, Y}(x, y)$<br />$\displaystyle P((X, Y)\in A) = \mathop{\iint}_{A}f_{X, Y}(x, y)dxdy$ |
| **Marginal** | $\displaystyle P(X=x) = \sum_yP(X=x, Y=y)$                   | $\displaystyle f_X(x) = \int^{\infty}_{-\infty}f_{X ,Y}(x, y)dy$ |
|   **Cond**   | $\displaystyle P(Y = y \mid X = x) = \frac{P(X = x, Y = y)}{P(X = x)}$ | $\displaystyle f_{Y \mid X}(y \mid x) = \frac{f_{X, Y}(x, y)}{f_X(x)} $ |
|  **Indep**   | $P(X = x, Y = y) = P(X = x)P(Y = y)$                         | $f_{X,Y}(x, y) = f_X(x)f_Y((y))$                             |

| Discrete $X \sim$                                    |                        PMF $P(X = k)$                        |              $E(X)$               |              $\text{Var}(X)$               |                     MGF $M(t)$                      |
| ---------------------------------------------------- | :----------------------------------------------------------: | :-------------------------------: | :----------------------------------------: | :-------------------------------------------------: |
| $\text{Bern}(p)$<br />One time                       | $\begin{aligned} k = 1 &\Rightarrow p \\ k = 0 &\Rightarrow 1-p \end{aligned}$ |                $p$                |                  $p(1-p)$                  |                   $pe^t + (1-p)$                    |
| $\text{Bin}(n, p)$<br />#S in $n$ trials             |              $\pmatrix{n \\ k}p^k(1- p)^{n-k}$               |               $np$                |                 $np(1-p)$                  |                 $(pe^t + (1-p))^n$                  |
| $\text{Geom}(p)$<br />#F before $1^{\text{st}}$ S    |                         $p(1 - p)^k$                         |   $\displaystyle \frac{1-p}{p}$   |      $\displaystyle \frac{1-p}{p^2}$       |        $\displaystyle \frac{p}{1-(1-p)e^t}$         |
| $\text{NBin}(r, p)$<br />#F before $r^{\text{th}}$ S |           $\pmatrix{k + r - 1 \\ r - 1}p^r(1-p)^k$           |  $\displaystyle r\frac{1-p}{p}$   |      $\displaystyle r\frac{1-p}{p^2}$      | $\displaystyle \left(\frac{p}{1-(1-p)e^t}\right)^r$ |
| $\text{HGeom}(w, b, n)$<br />#$w$ in chosen $n$      | $\displaystyle \frac{{w \choose k} {b \choose n-k}}{w + b \choose n}$ | $\displaystyle n \frac{w}{w + b}$ | $\displaystyle \frac{w+b-n}{w+b-1}np(1-p)$ |                      $\times$                       |
| $\text{Pois}(\lambda)$                               |       $\displaystyle\frac{e^{-\lambda}\lambda^k}{k!}$        |             $\lambda$             |                 $\lambda$                  |               $\exp (\lambda(e^t-1))$               |

| Continuous                                                   |                          PDF $f(x)$                          |                       CDF $F(x)$                        |              $E(X)$               |           $\text{Var}(X)$           |                        MGF $M(t)$                        |
| ------------------------------------------------------------ | :----------------------------------------------------------: | :-----------------------------------------------------: | :-------------------------------: | :---------------------------------: | :------------------------------------------------------: |
| $U \sim \text{Unif}(a, b)$                                   |               $\displaystyle \frac{1}{b - a}$                |             $\displaystyle \frac{x-a}{b-a}$             |   $\displaystyle \frac{a+b}{2}$   | $\displaystyle \frac{(b-a)^2}{12}$  |      $\displaystyle \frac{e^{tb} -e^{ta}}{t(b-a)}$       |
| $\mathcal{Z} \sim \mathcal{N}(0, 1)$                         | $\varphi(z) = \displaystyle \frac{1}{\sqrt{2 \pi}}e^{-z^2/2}$ |                        $\Phi(z)$                        |                $0$                |                 $1$                 |                       $e^{t^2/2}$                        |
| $X \sim \mathcal{N}(\mu, \sigma^2)$<br />$X = \mu + \sigma \mathcal{Z}$ | $\displaystyle \varphi\left(\frac{x - \mu}{\sigma}\right) \frac{1}{\sigma}$ | $\displaystyle \Phi\left(\frac{x - \mu}{\sigma}\right)$ |               $\mu$               |             $\sigma^2$              |           $e^{\mu t + \frac 1 2 \sigma^2t^2}$            |
| $X \sim \text{Expo}(\lambda)$<br />$\lambda X \sim \text{Expo}(1)$ |                       $e^{-\lambda x}$                       |                  $1 - e^{-\lambda x}$                   | $\displaystyle \frac{1}{\lambda}$ | $\displaystyle \frac{1}{\lambda^2}$ |       $\displaystyle \frac{\lambda}{\lambda - t}$        |
| $X \sim \text{Gamma}(a, \lambda)$<br />$\lambda X \sim \text{Gamma}(a, 1)$ | $\displaystyle \frac{1}{\Gamma(a)}(\lambda x)^ae^{-\lambda x}\frac{1}{x}$ |                        $\times$                         | $\displaystyle \frac{a}{\lambda}$ | $\displaystyle \frac{a}{\lambda^2}$ | $\displaystyle \left(\frac{\lambda}{\lambda-t}\right)^a$ |
| $X \sim \text{Beta}(a, b)$                                   |   $\displaystyle \frac{1}{\beta(a, b)}x^{a-1}(1-x)^{b-1}$    |                        $\times$                         |  $\displaystyle \frac{a}{a + b}$  |              $\times$               |                         $\times$                         |
